Runtime/Execution/Next.lean
@@ -8,25 +8,50 @@ def nextTime (exec : Executable net) : Option (Time.From exec.time) :=
   | none => none
   | some nextEvent => some ⟨nextEvent.time, exec.lawfulQueue h⟩
 
+theorem nextTime_some {exec : Executable net} {time} :
+  (exec.nextTime = some time) → (∃ event, exec.queue[0]? = some event ∧ event.time ≥ time.val) := by
+  intro h
+  unfold nextTime at h
+  split at h <;> simp at h
+  case _ event h' =>
+    exists event
+    apply And.intro h'
+    simp [←h]
+
 theorem nextTime_isSome_iff_queue_not_isEmpty {exec : Executable net} :
   exec.nextTime.isSome ↔ ¬exec.queue.isEmpty := by
   rw [←Array.getElem?_zero_isSome_iff_not_isEmpty]
   simp [nextTime]
   constructor <;> split <;> simp_all [Option.isSome]
 
+private def propagationEvents (exec : Executable net) :=
+  exec.toPropagate.uniqueMergeMap fun port =>
+    match exec.reactors port.reactor |>.interface .outputs port.port with
+    | none => #[] -- TODO: This case is unreachable by the semantics of `toPropagate`.
+    | some value =>
+      let events := port.delayedDestinations.map fun { dst, delay, eqType } =>
+        Event.propagation (exec.time + delay) dst (eqType ▸ value)
+      events.insertionSort (·.time ≤ ·.time) -- TODO: Use `qsort` when it drops `[Inhabited α]`.
+
+private theorem propagationEvents_LawfulQueue {exec : Executable net} {time} :
+  (LawfulQueue exec.propagationEvents time) := sorry
+  -- TODO: We need theorems about `Array.uniqueMergeMap/.map` to prove this.
+
 -- The first array are the next events to be executed at `time`.
 -- The second array is the remaining queue.
-private def eventSplit (exec : Executable net) (time : Time) : Array (Event net) × Array (Event net) :=
-  let ⟨candidates, later⟩ := exec.queue.split (·.time = time)
+private def eventSplit (queue : Array (Event net)) (time : Time) : Array (Event net) × Array (Event net) :=
+  let ⟨candidates, later⟩ := queue.split (·.time = time)
   let ⟨next, postponed⟩ := candidates.unique (·.id)
   (next, postponed ++ later)
 
-theorem eventSplit_fst_LawfulQueue {exec : Executable net} {time} :
-  LawfulQueue (exec.eventSplit time).fst time := sorry
+private theorem eventSplit_fst_LawfulQueue {queue : Array (Event net)} {time} :
+  (LawfulQueue queue time) →
+  (LawfulQueue (eventSplit queue time).fst time) := sorry
   -- TODO: We need theorems about `Array.unique/.split` to prove this.
 
-theorem eventSplit_snd_LawfulQueue {exec : Executable net} {time} :
-  LawfulQueue (exec.eventSplit time).snd time := sorry
+private theorem eventSplit_snd_LawfulQueue {queue : Array (Event net)} {time} :
+  (LawfulQueue queue time) →
+  (LawfulQueue (eventSplit queue time).snd time) := sorry
   -- TODO: We need theorems about `Array.unique/.split` to prove this.
 
 private def nextTimerEvents (exec : Executable net) (timers : Array (TimerId net)) (anchor : Time) : Array (Event net) :=
@@ -53,57 +78,51 @@ def empty (tag : Tag) : Next net where
   queue := #[]
   lawfulQueue := LawfulQueue.empty
 
--- UNFINISHED: Add propagation events.
-protected def «for» (exec : Executable net) (time : Time.From exec.time) : Next net :=
-  let eventSplit := exec.eventSplit time -- TODO: We can't destruct here, as this causes problems in the proof of `lawfulQueue`.
+protected def «for» (exec : Executable net) {time} (h : exec.nextTime = some time) : Next net :=
+  -- TODO: We can't destruct here, as this causes problems in the proof of `lawfulQueue`.
+  let eventSplit := eventSplit (exec.queue.merge exec.propagationEvents) time
   let events := eventSplit.fst
   let later := eventSplit.snd
   let timers := events.filterMap (·.timer?)
   let timerEvents := exec.nextTimerEvents timers time
   {
     tag         := exec.tag.advance time
+    events      := events
     queue       := later.merge timerEvents
-    lawfulQueue := (exec.tag.advance_time time) ▸ LawfulQueue.merge eventSplit_snd_LawfulQueue nextTimerEvents_LawfulQueue
-    events
+    lawfulQueue := by
+      rw [exec.tag.advance_time time]
+      refine LawfulQueue.merge ?_ nextTimerEvents_LawfulQueue
+      refine eventSplit_snd_LawfulQueue (LawfulQueue.merge ?_ propagationEvents_LawfulQueue)
+      have ⟨e, he, h'⟩ := nextTime_some h
+      intro event he'
+      simp [he] at he'
+      simp [←he', h']
   }
 
-/- For the UNFINISHED above:
-exec.toPropagate.uniqueMergeMap fun port =>
-  match output.raw.ports port with
-  | none => #[] -- TODO: This case is unreachable by the semantics of `toPropagate`.
-  | some value =>
-      parent.class.connections.delayed ⟨leaf, Path.split_class h₁ ▸ port'⟩ |>.map fun ⟨delay, dst⟩ =>
-        let input : InputPortId net := {
-          reactor := parent.extend dst.child
-          port := sorry -- dst.port
-        }
-        have H : input.reactor.inputs.type input.port = output.reaction.val.portEffects.type port := sorry
-        Event.propagation (exec.time + delay) input (H ▸ value)
--/
-
-theorem for_preserves_events {time} : (Next.for exec time = next) → ∃ timerEvents, (next.events ++ next.queue) ~ (exec.queue ++ timerEvents) := by
-  intro h
-  simp [Next.for] at h
-  let events := (exec.eventSplit time).fst
-  let timers := events.filterMap (·.timer?)
-  exists exec.nextTimerEvents timers time
+theorem for_preserves_events :
+  (Next.for exec h = next) →
+  ∃ timerEvents propagationEvents,
+    (next.events ++ next.queue) ~ (exec.queue ++ timerEvents ++ propagationEvents) := by
   sorry
 
 -- The actions-interface for a given reactor according to the `Next` instance.
-def actions (next : Next net) (reactor : ReactorId net) : Interface? (reactor.class.interface .actions) :=
+def actions (next : Next net) (reactor : ReactorId net) :
+  Interface? (reactor.class.interface .actions) :=
   fun action =>
     match h : next.events.findP? (·.id = .action ⟨reactor, action⟩) with
-    | none => none
+    | none       => none
     | some event => have h := Array.findP?_property h; event.actionValue (of_decide_eq_true h)
 
 -- The inputs-interface for a given reactor according to the `Next` instance.
-def inputs (next : Next net) (reactor : ReactorId net) : Interface? (reactor.class.interface .inputs) :=
+def inputs (next : Next net) (reactor : ReactorId net) :
+  Interface? (reactor.class.interface .inputs) :=
   fun input =>
     match h : next.events.findP? (·.id = .propagation ⟨reactor, input⟩) with
     | none => none
     | some event => have h := Array.findP?_property h; event.propagationValue (of_decide_eq_true h)
 
-def timers (next : Next net) (exec : Executable net) (reactor : ReactorId net) : reactor.class.timers → Reactor.Timer :=
+def timers (next : Next net) (exec : Executable net) (reactor : ReactorId net) :
+  reactor.class.timers → Reactor.Timer :=
   fun timer => {
     val      := exec.reactors reactor |>.timer timer |>.val
     isFiring := next.events.any (·.timer? = some ⟨reactor, timer⟩)
