Runtime/Network/Basic.lean
@@ -43,7 +43,7 @@ structure ReactionId (net : Network) where
 abbrev ReactionId.reaction (id : ReactionId net) :=
   id.reactor.class.reactions[id.reactionIdx]
 
-def ReactionId.affects (id : ReactionId net) (port : (id.reactor.class.interface .outputs).vars) : Bool :=
+def ReactionId.affects (id : ReactionId net) (port : (id.reactor.outputs).vars) : Bool :=
   id.reaction.subPE.inv (.inl port) |>.isSome
 
 structure TimerId (net : Network) where
@@ -55,5 +55,47 @@ structure PortId (net : Network) (kind : Reactor.PortKind) where
   reactor : ReactorId net
   port    : reactor.class.interface kind |>.vars
   deriving DecidableEq
+
+def PortId.hasDelayedConnection (port : PortId net .output) : Bool :=
+  if h : port.reactor.isCons then
+    -- TODO: We can't destruct here because then the type cast on `port.port` doesn't work.
+    let split := port.reactor.split h
+    let parent := split.fst
+    let leaf := split.snd
+    ¬ (parent.class.connections.delayed ⟨leaf, Path.split_class h ▸ port.port⟩ |>.isEmpty)
+  else
+    -- In this case the reaction that produced the output lives in the top level reactor,
+    -- so there are no connections.
+    false
+
+structure PortId.DelayedDestination (port : PortId net .output) where
+  dst : PortId net .input
+  delay : Duration
+  eqType : (port.reactor.outputs).type port.port = (dst.reactor.inputs).type dst.port
+
+open Path in
+def PortId.delayedDestinations (port : PortId net .output) : Array (DelayedDestination port) :=
+  if h : port.reactor.isCons then
+    -- TODO: We can't destruct here because then the type cast on `port` doesn't work.
+    let split := port.reactor.split h
+    let parent := split.fst
+    let leaf := split.snd
+    let src := ⟨leaf, split_class h ▸ port.port⟩
+    parent.class.connections.delayed src |>.map fun { dst, delay, eqType } => {
+      delay := delay
+      dst := ⟨parent.extend dst.child, extend_class ▸ dst.port⟩
+      eqType := by
+        have h₁ := eqType
+        have h₂ := split_class h
+        have h₃ := extend_class (path := parent) (leaf := leaf)
+        -- TODO: h₁, h₂ and h₃ should suffice to show the theorem.
+        --       The problem is just simultaneous rewriting again.
+        simp
+        sorry
+    }
+  else
+    -- In this case the reaction that produced the output lives in the top level reactor,
+    -- so there are no connections and hence no destinations.
+    #[]
 
 end Network
